toy2.v
@@ -3,58 +3,99 @@ From iris.heap_lang Require Export lifting notation locations lang.
 From iris.base_logic.lib Require Export invariants.
 From iris.program_logic Require Export atomic.
 From iris.proofmode Require Import tactics.
-From iris.heap_lang Require Import proofmode notation par.
+From iris.heap_lang Require Import proofmode atomic_heap notation par.
 From iris.bi.lib Require Import fractional.
 From iris.bi Require Import derived_laws_sbi.
 Set Default Proof Using "Type*".
 
 Definition lockNode : val :=
-  rec: "lockN" "x" :=
+  rec: "lockN" "y" :=
     if: CAS "y" #false #true
     then #()
-    else "lockN" "x".
+    else "lockN" "y".
 
 Definition unlockNode : val :=
-  λ: "x",
+  λ: "y",
   "y" <- #false.
 
 Definition prog : val := 
-  λ: "x" "v",
-  lockNode "x";;
+  λ: "x" "y" "v",
+  lockNode "y";;
   "x" <- "v";;
-  unlockNode "x";; "v".
+  unlockNode "y";; "v".
 
 Section Toy_Template.
   Context `{!heapG Σ} (N : namespace).
   Notation iProp := (iProp Σ).
 
-(*
-  Definition toyN : namespace := N .@ "toy".
+  (* We should be able to prove the following specs: *)
 
-  Definition main_inv x y (b: bool) d := (y ↦ #b ∗ if b then True else x ↦ d)%I.
-
-  Definition is_toy x y := inv toyN (∃ b d, main_inv x y b d)%I.
-
-  Instance main_inv_timeless x y b d: Timeless (main_inv x y b d).
+  Lemma lock_spec (y: loc) :
+    <<< ∀ (b: bool), y ↦ #b >>>
+        lockNode #y @ ⊤
+    <<< y ↦ #true ∗ if b then False else True, RET #() >>>.
   Proof.
-    rewrite /main_inv. repeat apply bi.sep_timeless; try apply _.
-    destruct b; try apply _.
-  Qed.
+    iIntros (Φ) "AU". wp_lam.
+    wp_bind(CmpXchg _ _ _)%E.
+(* ***** This is where I get the error ***** *)
+(*     awp_apply (cmpxchg_spec y #false #true). *)
+  Admitted.
 
-  Lemma lockNode_spec (x y: loc):
-      is_toy x y -∗
-      <<< True >>> lockNode #x @ ⊤∖↑toyN <<< y ↦ #true, RET #() >>>.
+  Lemma unlock_spec (y: loc) :
+    <<< y ↦ #true >>>
+        unlockNode #y @ ⊤
+    <<< y ↦ #false, RET #() >>>.
+  Proof. Admitted.
+
+  Definition is_locked_ref x y v : iProp :=
+    (∃ (b: bool), y ↦ #b ∗ if b then True else x ↦ v)%I.
+
+  Lemma prog_spec (x y: loc) (v: val) :
+    <<< ∀ (u: val), is_locked_ref x y u >>>
+        prog #x #y v @ ⊤
+    <<< is_locked_ref x y v, RET #() >>>.
   Proof.
-    iIntros "#HInv" (Φ) "AU". iLöb as "IH".
-    wp_lam. wp_bind (CmpXchg _ _ _)%E.
-    iInv "HInv" as "HI".
-*)
-
-  Definition main_inv x y := (∃ (b:bool) d, y ↦ #b ∗ if b then True else x ↦ d)%I.
-
-  Lemma lockNode_spec (x y: loc):
-      <<< main_inv x y >>> lockNode #x @ ⊤ <<< main_inv x y ∗ y ↦ #true, RET #() >>>.
-  Proof.
-    iIntros (Φ) "AU". iLöb as "IH".
-    wp_lam. wp_bind (CmpXchg _ _ _)%E.
-    iMod "AU" as "[hoho [_ HClose]]".
+    unfold is_locked_ref.
+    iIntros (Φ) "HP". iLöb as "IH".
+    wp_lam. wp_pures. wp_bind (lockNode _)%E.
+(*  atomic spec for lock  *)
+    awp_apply (lock_spec).
+(* peeking into the AU *)
+    iApply (aacc_aupd_abort with "HP"). done.
+    iIntros (v0) "Hislock". 
+    iDestruct "Hislock" as (b) "(Hy & Hif)".
+    iAaccIntro with "Hy".
+(* the atomic lock_spec either aborts or commits, which are the two cases below *)
+    - (* abort *)
+      iIntros "Hy". iModIntro.
+      iSplitL. iExists b. iFrame.
+      eauto with iFrame.
+    - (* commit, below is the post-condition of lock_spec *)
+      iIntros "(Hy & Hif')".
+      destruct (b).
+      + iExFalso. done.
+      + iModIntro.
+        (* left-most spatial proposition is giving back the AU, after peeking *)
+        iSplitR "Hif". 
+        (* here is where we give away y ↦ #true *)
+        iExists true. iFrame.
+        iIntros "HP". iModIntro.
+        wp_pures. wp_store.
+        awp_apply (unlock_spec).
+        (* need y ↦ #true to open the atomic accessor (AACC thing), but we don't have,
+           we can peek into the AU again, but that does not give us y ↦ #true, just y ↦ some b *)
+        iApply (aacc_aupd_abort with "HP"). done.
+        iIntros (v1) "Hislock".
+        iDestruct "Hislock" as (b') "(Hy & H')".
+(*  At this point, we need y ↦ #true, but we don't have that information.
+    This is because when we apply the lock_spec, we need y ↦ _ for the 
+    lock_spec, which we obtain by peeking into the AU. That gives us is_locked_ref
+    (and y ↦ _) but we have to give back is_locked_ref after the atomic step. At that point,
+    we have y ↦ #true from the post-condition of the lock_spec, but we 
+    have to use it to give bakc is_locked_ref. When we have to unlock later,
+    we thus does not have y ↦ #true, which is required by the pre-condition
+    of unlock_spec. In this scenario, I think what we may work is fractional
+    mapping, of the form y ↦{1/2} _. One-half belongs in the spec, the other half in the
+    is_locked_ref. The store is allowed only if we have the full ownership, which
+    we will by writing appropriate specs for lock and unlock.
+    Hope this makes sense, haha!     *)
